src/Functional.v
@@ -49,115 +49,115 @@ Section bisim.
   | Modify : forall (f : C -> C), ModifyE C
   .
 
-  Definition E (C : Type) := (exceptE unit +' @ModifyE C +' nondetE).
+  Definition sceE (C : Type) := (exceptE unit +' @ModifyE C +' nondetE).
 
   Context {config specConfig : Type}.
 
-  Variant no_error_gen {R C : Type} no_error (c : C) : itree (E C) R -> Prop :=
-  | no_error_ret : forall r, no_error_gen no_error c (Ret r)
-  | no_error_tau : forall t, no_error c t -> no_error_gen no_error c (Tau t)
-  | no_error_modify : forall f k,
-      no_error (f c) (k c) ->
-      no_error_gen no_error c (vis (Modify f) k)
-  | no_error_choice : forall k,
-      (forall b, no_error c (k b)) ->
-      no_error_gen no_error c (vis Or k)
+  Variant no_errors_gen {R C : Type} no_errors (c : C) : itree (sceE C) R -> Prop :=
+  | no_errors_ret : forall r, no_errors_gen no_errors c (Ret r)
+  | no_errors_tau : forall t, no_errors c t -> no_errors_gen no_errors c (Tau t)
+  | no_errors_modify : forall f k,
+      no_errors (f c) (k c) ->
+      no_errors_gen no_errors c (vis (Modify f) k)
+  | no_errors_choice : forall k,
+      (forall b, no_errors c (k b)) ->
+      no_errors_gen no_errors c (vis Or k)
   .
 
-  Definition no_error {R C : Type} :=
-    paco2 (@no_error_gen R C) bot2.
+  Definition no_errors {R C : Type} :=
+    paco2 (@no_errors_gen R C) bot2.
 
-  Lemma no_error_gen_mon {R C} : monotone2 (@no_error_gen R C).
+  Lemma no_errors_gen_mon {R C} : monotone2 (@no_errors_gen R C).
   Proof.
     repeat intro. inversion IN; subst; try solve [constructor; auto].
   Qed.
-  Hint Resolve no_error_gen_mon : paco.
+  Hint Resolve no_errors_gen_mon : paco.
 
   Program Definition eq_p {T : Type} (y x : T) : (@Perms (config * specConfig)) :=
   {|
   in_Perms := fun _ => x = y;
   |}.
 
-  Inductive typing_gen {R1 R2 : Type} (typing : perm -> (R1 -> R2 -> Perms) -> itree (E config) R1 -> config -> itree (E specConfig) R2 -> specConfig -> Prop)
+  Inductive sbuter_gen {R1 R2 : Type} (sbuter : perm -> (R1 -> R2 -> Perms) -> itree (sceE config) R1 -> config -> itree (sceE specConfig) R2 -> specConfig -> Prop)
             (p : perm) (Q : R1 -> R2 -> Perms) :
-    itree (E config) R1 -> config -> itree (E specConfig) R2 -> specConfig -> Prop :=
-  | typing_gen_ret r1 c1 r2 c2 :
+    itree (sceE config) R1 -> config -> itree (sceE specConfig) R2 -> specConfig -> Prop :=
+  | sbuter_gen_ret r1 c1 r2 c2 :
       pre p (c1, c2) ->
       p ∈ Q r1 r2 ->
-      typing_gen typing p Q (Ret r1) c1 (Ret r2) c2
-  | typing_gen_err t1 c1 c2 :
-      typing_gen typing p Q t1 c1 (throw tt) c2
-  | typing_gen_tau_L t1 c1 t2 c2 :
+      sbuter_gen sbuter p Q (Ret r1) c1 (Ret r2) c2
+  | sbuter_gen_err t1 c1 c2 :
+      sbuter_gen sbuter p Q t1 c1 (throw tt) c2
+  | sbuter_gen_tau_L t1 c1 t2 c2 :
       pre p (c1, c2) ->
-      typing_gen typing p Q t1 c1 t2 c2 ->
-      typing_gen typing p Q (Tau t1) c1 t2 c2
-  | typing_gen_tau_R t1 c1 t2 c2 :
+      sbuter_gen sbuter p Q t1 c1 t2 c2 ->
+      sbuter_gen sbuter p Q (Tau t1) c1 t2 c2
+  | sbuter_gen_tau_R t1 c1 t2 c2 :
       pre p (c1, c2) ->
-      typing_gen typing p Q t1 c1 t2 c2 ->
-      typing_gen typing p Q t1 c1 (Tau t2) c2
-  | typing_gen_tau t1 c1 t2 c2 :
+      sbuter_gen sbuter p Q t1 c1 t2 c2 ->
+      sbuter_gen sbuter p Q t1 c1 (Tau t2) c2
+  | sbuter_gen_tau t1 c1 t2 c2 :
       pre p (c1, c2) ->
-      typing p Q t1 c1 t2 c2 ->
-      typing_gen typing p Q (Tau t1) c1 (Tau t2) c2
-  | typing_gen_modify_L f k c1 t2 c2 p' :
+      sbuter p Q t1 c1 t2 c2 ->
+      sbuter_gen sbuter p Q (Tau t1) c1 (Tau t2) c2
+  | sbuter_gen_modify_L f k c1 t2 c2 p' :
       pre p (c1, c2) ->
       guar p (c1, c2) (f c1, c2) ->
       sep_step p p' ->
-      typing_gen typing p' Q (k c1) (f c1) t2 c2 ->
-      typing_gen typing p Q (vis (Modify f) k) c1 t2 c2
-  | typing_gen_modify_R t1 c1 f k c2 p' :
+      sbuter_gen sbuter p' Q (k c1) (f c1) t2 c2 ->
+      sbuter_gen sbuter p Q (vis (Modify f) k) c1 t2 c2
+  | sbuter_gen_modify_R t1 c1 f k c2 p' :
       pre p (c1, c2) ->
       guar p (c1, c2) (c1, f c2) ->
       sep_step p p' ->
-      typing_gen typing p' Q t1 c1 (k c2) (f c2) ->
-      typing_gen typing p Q t1 c1 (vis (Modify f) k) c2
-  | typing_gen_modify f1 k1 c1 f2 k2 c2 p' :
+      sbuter_gen sbuter p' Q t1 c1 (k c2) (f c2) ->
+      sbuter_gen sbuter p Q t1 c1 (vis (Modify f) k) c2
+  | sbuter_gen_modify f1 k1 c1 f2 k2 c2 p' :
       pre p (c1, c2) ->
       guar p (c1, c2) (f1 c1, f2 c2) ->
       sep_step p p' ->
-      typing p' Q (k1 c1) (f1 c1) (k2 c2) (f2 c2) ->
-      typing_gen typing p Q (vis (Modify f1) k1) c1 (vis (Modify f2) k2) c2
-  | typing_gen_choice_L k c1 t2 c2 p' :
+      sbuter p' Q (k1 c1) (f1 c1) (k2 c2) (f2 c2) ->
+      sbuter_gen sbuter p Q (vis (Modify f1) k1) c1 (vis (Modify f2) k2) c2
+  | sbuter_gen_choice_L k c1 t2 c2 p' :
       pre p (c1, c2) ->
       sep_step p p' ->
-      (forall b, typing_gen typing p' Q (k b) c1 t2 c2) ->
-      typing_gen typing p Q (vis Or k) c1 t2 c2
-  | typing_gen_choice_R t1 c1 k c2 p' :
+      (forall b, sbuter_gen sbuter p' Q (k b) c1 t2 c2) ->
+      sbuter_gen sbuter p Q (vis Or k) c1 t2 c2
+  | sbuter_gen_choice_R t1 c1 k c2 p' :
       pre p (c1, c2) ->
       sep_step p p' ->
-      (forall b, typing_gen typing p' Q t1 c1 (k b) c2) ->
-      typing_gen typing p Q t1 c1 (vis Or k) c2
-  | typing_gen_choice k1 c1 k2 c2 p' :
+      (forall b, sbuter_gen sbuter p' Q t1 c1 (k b) c2) ->
+      sbuter_gen sbuter p Q t1 c1 (vis Or k) c2
+  | sbuter_gen_choice k1 c1 k2 c2 p' :
       pre p (c1, c2) ->
       sep_step p p' ->
-      (forall b1, exists b2, typing p' Q (k1 b1) c1 (k2 b2) c2) ->
-      (forall b2, exists b1, typing p' Q (k1 b1) c1 (k2 b2) c2) ->
-      typing_gen typing p Q (vis Or k1) c1 (vis Or k2) c2
+      (forall b1, exists b2, sbuter p' Q (k1 b1) c1 (k2 b2) c2) ->
+      (forall b2, exists b1, sbuter p' Q (k1 b1) c1 (k2 b2) c2) ->
+      sbuter_gen sbuter p Q (vis Or k1) c1 (vis Or k2) c2
   .
 
-  Lemma typing_gen_mon {R1 R2} : monotone6 (@typing_gen R1 R2).
+  Lemma sbuter_gen_mon {R1 R2} : monotone6 (@sbuter_gen R1 R2).
   Proof.
     repeat intro. induction IN; subst; try solve [econstructor; eauto]; auto.
     econstructor 11; eauto; intros.
     - destruct (H1 b1). eexists; eauto.
     - destruct (H2 b2). eexists; eauto.
   Qed.
-  Hint Resolve typing_gen_mon : paco.
+  Hint Resolve sbuter_gen_mon : paco.
 
-  Definition typing_ {R1 R2} := paco6 (@typing_gen R1 R2) bot6.
+  Definition sbuter {R1 R2} := paco6 (@sbuter_gen R1 R2) bot6.
 
-  Lemma typing_gen_pre {R1 R2} r p (Q : R1 -> R2 -> Perms) t s c1 c2 :
-    typing_gen r p Q t c1 s c2 ->
+  Lemma sbuter_gen_pre {R1 R2} r p (Q : R1 -> R2 -> Perms) t s c1 c2 :
+    sbuter_gen r p Q t c1 s c2 ->
     s = throw tt \/ pre p (c1, c2).
   Proof.
     inversion 1; auto.
   Qed.
 
-  Definition typing {R1 R2} P Q (t : itree (E config) R1) (s : itree (E specConfig) R2) :=
-    forall p c1 c2, p ∈ P -> pre p (c1, c2) -> typing_ p Q t c1 s c2.
+  Definition typing {R1 R2} P Q (t : itree (sceE config) R1) (s : itree (sceE specConfig) R2) :=
+    forall p c1 c2, p ∈ P -> pre p (c1, c2) -> sbuter p Q t c1 s c2.
 
-  Lemma typing_lte' {R1 R2} p Q Q' (t : itree (E config) R1) (s : itree (E specConfig) R2) c1 c2 :
-    typing_ p Q t c1 s c2 -> (forall r1 r2, Q r1 r2 ⊦ Q' r1 r2) -> typing_ p Q' t c1 s c2.
+  Lemma sbuter_lte {R1 R2} p Q Q' (t : itree (sceE config) R1) (s : itree (sceE specConfig) R2) c1 c2 :
+    sbuter p Q t c1 s c2 -> (forall r1 r2, Q r1 r2 ⊦ Q' r1 r2) -> sbuter p Q' t c1 s c2.
   Proof.
     revert p Q Q' t s c1 c2. pcofix CIH. intros p Q Q' t s c1 c2 Htyping Hlte.
     punfold Htyping. pstep.
@@ -168,14 +168,14 @@ Section bisim.
       + destruct (H2 b2). eexists. right. eapply CIH; eauto. pclearbot. apply H3.
   Qed.
 
-  Lemma typing_lte {R1 R2} P P' Q Q' (t : itree (E config) R1) (s : itree (E specConfig) R2) :
+  Lemma typing_lte {R1 R2} P P' Q Q' (t : itree (sceE config) R1) (s : itree (sceE specConfig) R2) :
     typing P Q t s ->
     P' ⊦ P ->
     (forall r1 r2, Q r1 r2 ⊦ Q' r1 r2) ->
     typing P' Q' t s.
   Proof.
     repeat intro.
-    eapply typing_lte'; eauto.
+    eapply sbuter_lte; eauto.
   Qed.
 
   Lemma typing_ret {R1 R2} P Q (r1 : R1) (r2 : R2) :
@@ -193,21 +193,21 @@ Section bisim.
 
 
   Lemma typing_spin {R1 R2} P Q :
-    typing P Q (ITree.spin : itree (E config) R1) (ITree.spin : itree (E specConfig) R2).
+    typing P Q (ITree.spin : itree (sceE config) R1) (ITree.spin : itree (sceE specConfig) R2).
   Proof.
     repeat intro. pcofix CIH. pstep.
     rewrite (@rewrite_spin _ R1). rewrite (@rewrite_spin _ R2).
     constructor 5; auto.
   Qed.
 
-  Lemma typing_top {R1 R2} Q (t : itree (E config) R1) (s : itree (E specConfig) R2) :
+  Lemma typing_top {R1 R2} Q (t : itree (sceE config) R1) (s : itree (sceE specConfig) R2) :
     typing top_Perms Q t s.
   Proof.
     repeat intro. inversion H.
   Qed.
 
-  Lemma typing_bottom' {R1 R2} p Q (t : itree (E config) R1) (s : itree (E specConfig) R2) c1 c2:
-    typing_ p Q t c1 s c2 -> typing_ p (fun _ _ => bottom_Perms) t c1 s c2.
+  Lemma sbuter_bottom {R1 R2} p Q (t : itree (sceE config) R1) (s : itree (sceE specConfig) R2) c1 c2:
+    sbuter p Q t c1 s c2 -> sbuter p (fun _ _ => bottom_Perms) t c1 s c2.
   Proof.
     revert p Q t s c1 c2. pcofix CIH. intros. pstep. punfold H0.
     induction H0; pclearbot; try solve [econstructor; simpl; eauto].
@@ -216,20 +216,20 @@ Section bisim.
     - destruct (H2 b2). eexists. right. eapply CIH; pclearbot; apply H3.
   Qed.
 
-  Lemma typing_bottom {R1 R2} P Q (t : itree (E config) R1) (s : itree (E specConfig) R2) :
+  Lemma typing_bottom {R1 R2} P Q (t : itree (sceE config) R1) (s : itree (sceE specConfig) R2) :
     typing P Q t s -> typing P (fun _ _ => bottom_Perms) t s.
   Proof.
-    repeat intro. eapply typing_bottom'; eauto.
+    repeat intro. eapply sbuter_bottom; eauto.
   Qed.
 
-  Lemma typing_bind' {R1 R2 S1 S2} (p : perm) (Q : R1 -> S1 -> Perms) (R : R2 -> S2 -> Perms)
-        (t1 : itree (E config) R1) (t2 : R1 -> itree (E config) R2)
-        (s1 : itree (E specConfig) S1) (s2 : S1 -> itree (E specConfig) S2)
+  Lemma sbuter_bind {R1 R2 S1 S2} (p : perm) (Q : R1 -> S1 -> Perms) (R : R2 -> S2 -> Perms)
+        (t1 : itree (sceE config) R1) (t2 : R1 -> itree (sceE config) R2)
+        (s1 : itree (sceE specConfig) S1) (s2 : S1 -> itree (sceE specConfig) S2)
         c1 c2 :
     pre p (c1, c2) ->
-    typing_ p Q t1 c1 s1 c2 ->
+    sbuter p Q t1 c1 s1 c2 ->
     (forall r1 r2, typing (Q r1 r2) R (t2 r1) (s2 r2)) ->
-    typing_ p R (x <- t1 ;; t2 x) c1 (x <- s1 ;; s2 x) c2.
+    sbuter p R (x <- t1 ;; t2 x) c1 (x <- s1 ;; s2 x) c2.
   Proof.
     revert p Q R t1 t2 s1 s2 c1 c2. pcofix CIH.
     intros p Q R t1 t2 s1 s2 c1 c2 Hpre Htyping1 Htyping2.
@@ -245,51 +245,51 @@ Section bisim.
       pstep. constructor; auto.
     - do 2 rewritebisim @bind_tau. pclearbot.
       pstep. constructor 5; auto. right. eapply CIH; eauto.
-    - rewritebisim @bind_vis. apply typing_gen_pre in Htyping1. destruct Htyping1; subst.
+    - rewritebisim @bind_vis. apply sbuter_gen_pre in Htyping1. destruct Htyping1; subst.
       + rewrite throw_bind. pstep. constructor.
       + specialize (IHHtyping1 H2 Htyping2). punfold IHHtyping1. pstep. econstructor; eauto.
-    - rewritebisim @bind_vis. apply typing_gen_pre in Htyping1. destruct Htyping1; subst.
+    - rewritebisim @bind_vis. apply sbuter_gen_pre in Htyping1. destruct Htyping1; subst.
       + pstep. econstructor; eauto. rewrite H2. rewrite throw_bind. constructor.
       + specialize (IHHtyping1 H2 Htyping2). punfold IHHtyping1. pstep. econstructor; eauto.
     - do 2 rewritebisim @bind_vis. pclearbot.
       pose proof H2. punfold H2.
       pstep. econstructor 8; eauto.
-      destruct (typing_gen_pre _ _ _ _ _ _ _ H2); eauto.
+      destruct (sbuter_gen_pre _ _ _ _ _ _ _ H2); eauto.
       rewrite H4. rewrite throw_bind. left. pstep. constructor.
     - rewritebisim @bind_vis. pstep. econstructor; eauto. intros.
-      destruct (typing_gen_pre _ _ _ _ _ _ _ (H1 b)).
+      destruct (sbuter_gen_pre _ _ _ _ _ _ _ (H1 b)).
       + rewrite H3. rewrite throw_bind. constructor.
       + specialize (H2 b H3 Htyping2). punfold H2.
     - rewritebisim @bind_vis. pstep. econstructor; eauto. intros.
-      destruct (typing_gen_pre _ _ _ _ _ _ _ (H1 b)).
+      destruct (sbuter_gen_pre _ _ _ _ _ _ _ (H1 b)).
       + rewrite H3. rewrite throw_bind. constructor.
       + specialize (H2 b H3 Htyping2). punfold H2.
     - do 2 rewritebisim @bind_vis. pclearbot. pstep. econstructor 11; eauto; intros.
       + specialize (H1 b1). destruct H1. pclearbot.
-        punfold H1. destruct (typing_gen_pre _ _ _ _ _ _ _ H1).
+        punfold H1. destruct (sbuter_gen_pre _ _ _ _ _ _ _ H1).
         * exists x. left. pstep. rewrite H3. rewrite throw_bind. econstructor; eauto.
         * eexists. right. eapply CIH; eauto. pstep; eauto.
       + specialize (H2 b2). destruct H2. pclearbot.
-        punfold H2. destruct (typing_gen_pre _ _ _ _ _ _ _ H2).
+        punfold H2. destruct (sbuter_gen_pre _ _ _ _ _ _ _ H2).
         * exists x. left. pstep. rewrite H3. rewrite throw_bind. econstructor; eauto.
         * eexists. right. eapply CIH; eauto. pstep; eauto.
   Qed.
 
   Lemma typing_bind {R1 R2 S1 S2} (P : Perms) (Q : R1 -> S1 -> Perms) (R : R2 -> S2 -> Perms)
-        (t1 : itree (E config) R1) (t2 : R1 -> itree (E config) R2)
-        (s1 : itree (E specConfig) S1) (s2 : S1 -> itree (E specConfig) S2) :
+        (t1 : itree (sceE config) R1) (t2 : R1 -> itree (sceE config) R2)
+        (s1 : itree (sceE specConfig) S1) (s2 : S1 -> itree (sceE specConfig) S2) :
     typing P Q t1 s1 ->
     (forall r1 r2, typing (Q r1 r2) R (t2 r1) (s2 r2)) ->
     typing P R (x <- t1 ;; t2 x) (x <- s1 ;; s2 x).
   Proof.
     repeat intro.
-    eapply typing_bind'; eauto.
+    eapply sbuter_bind; eauto.
   Qed.
 
-  Lemma typing_soundness {R1 R2} Q (t : itree (E config) R1) (s : itree (E specConfig) R2) p c1 c2 :
-    typing_ p Q t c1 s c2 ->
-    no_error c2 s ->
-    no_error c1 t.
+  Lemma sbuter_no_errors {R1 R2} Q (t : itree (sceE config) R1) (s : itree (sceE specConfig) R2) p c1 c2 :
+    sbuter p Q t c1 s c2 ->
+    no_errors c2 s ->
+    no_errors c1 t.
   Proof.
     revert Q t s p c1 c2. pcofix CIH. intros Q t s p c1 c2 Htyping Hs. pstep.
     punfold Htyping.
@@ -309,7 +309,7 @@ Section bisim.
            (pointwise_relation _ (pointwise_relation _ eq_Perms)) ==> eq ==> eq ==> flip impl) (@typing R1 R2).
   Proof.
     repeat intro. subst.
-    eapply typing_lte'; eauto. apply H3; auto. rewrite <- H; auto.
+    eapply sbuter_lte; eauto. apply H3; auto. rewrite <- H; auto.
     intros. rewrite H0. reflexivity.
   Qed.
 End bisim.
